library/init/data/rbtree/lemmas.lean
@@ -12,7 +12,7 @@ universes u v
 local attribute [-simp] or.comm or.left_comm or.assoc
 
 namespace tactic
-/- TODO(Leo): move blast_disjs to another file. -/
+/- TODO(Leo): move blast_disjs and twice to another file. -/
 private meta def blast_disjs_aux : list expr → tactic unit
 | []      := failed
 | (h::hs) := do
@@ -27,6 +27,9 @@ namespace interactive
 meta def blast_disjs : tactic unit :=
 focus1 $ repeat $ any_goals $ local_context >>= blast_disjs_aux
 
+meta def twice (t : itactic) : tactic unit :=
+t >> t
+
 end interactive
 end tactic
 
@@ -37,47 +40,7 @@ open color nat
 
 def lift (lt : α → α → Prop) : option α → option α → Prop
 | (some a) (some b) := lt a b
-| none     (some b) := true
-| _         _       := false
-
-instance lift_lt_trans (lt : α → α → Prop) [is_trans α lt] : is_trans (option α) (lift lt) :=
-begin
-  constructor,
-  intros a b c,
-  cases a with a; cases b with b; cases c with c; simp [lift],
-  apply trans_of lt
-end
-
-instance lift_lt_irrefl (lt : α → α → Prop) [is_irrefl α lt] : is_irrefl (option α) (lift lt) :=
-begin
-  constructor,
-  intros a, cases a; simp [lift],
-  apply irrefl_of lt
-end
-
-instance lift_lt_incomp_trans (lt : α → α → Prop) [is_incomp_trans α lt] : is_incomp_trans (option α) (lift lt) :=
-begin
-  constructor,
-  intros a b c, cases a; cases b; cases c; simp [lift],
-  apply incomp_trans_of lt
-end
-
-instance (lt : α → α → Prop) [is_strict_weak_order α lt] : is_strict_weak_order (option α) (lift lt) :=
-{ trans        := λ a b c, trans_of (lift lt),
-  irrefl       := irrefl_of (lift lt),
-  incomp_trans := λ a b c, incomp_trans_of (lift lt) }
-
-instance (lt : α → α → Prop) [h : decidable_rel lt] : decidable_rel (lift lt)
-| none     none     := is_false not_false
-| none     (some b) := is_true trivial
-| (some a) none     := is_false not_false
-| (some a) (some b) := h a b
-
-lemma lift_lt_of_lt (lt : α → α → Prop) : ∀ {a b}, lt a b → lift lt (some a) (some b) :=
-begin simp [lift], intros, assumption end
-
-lemma not_lift_lt_of_not_lt (lt : α → α → Prop) : ∀ {a b}, ¬ lt a b → ¬ lift lt (some a) (some b) :=
-begin simp [lift], intros, assumption end
+| _         _       := true
 
 inductive is_searchable (lt : α → α → Prop) : rbnode α → option α → option α → Prop
 | leaf_s  {lo hi}       : lift lt lo hi → is_searchable leaf lo hi
@@ -95,7 +58,8 @@ begin
     cases h,
     have h₁ := ih_1 ‹is_searchable lt lchild lo (some val)›,
     have h₂ := ih_2 ‹is_searchable lt rchild (some val) hi›,
-    apply trans_of (lift lt) h₁ h₂
+    cases lo with lo; cases hi with hi; simp [lift] at *,
+    apply trans_of lt h₁ h₂,
   }
 end
 
@@ -114,20 +78,29 @@ begin
       cases h₃ with lo_x x_val,
       split,
       show lift lt lo (some x), { assumption },
-      show lift lt (some x ) hi, { apply trans_of (lift lt) x_val val_hi },
+      show lift lt (some x ) hi, {
+        cases hi with hi; simp [lift] at *,
+        apply trans_of lt x_val val_hi
+      }
     },
     {
       simp at h₂, cases h₂,
+      cases lo with lo; cases hi with hi; simp [lift] at *,
+      { apply lt_of_incomp_of_lt _ val_hi, simp [*] },
+      { apply lt_of_lt_of_incomp lo_val, simp [*] },
       split,
-      { apply lt_of_lt_of_incomp lo_val, split, repeat { assumption } },
-      { apply lt_of_incomp_of_lt _ val_hi, split, repeat { assumption }  }
+      { apply lt_of_incomp_of_lt _ val_hi, simp [*] },
+      { apply lt_of_lt_of_incomp lo_val, simp [*] }
     },
     {
       have h₃ : lift lt (some val) (some x) ∧ lift lt (some x) hi, { apply ih_2, assumption, assumption },
       cases h₃ with val_x x_hi,
+      cases lo with lo; cases hi with hi; simp [lift] at *,
+      { assumption },
+      { apply trans_of lt lo_val val_x },
       split,
-      show lift lt lo (some x), { apply trans_of (lift lt) lo_val val_x },
-      show lift lt (some x) hi, { assumption }
+      { assumption },
+      { apply trans_of lt lo_val val_x, }
     }
   }
 end
@@ -166,46 +139,40 @@ lemma contains_correct {t : rbnode α} {lt x} [decidable_rel lt] [is_strict_weak
 begin
   apply contains.induction lt t x; intros; simp only [mem, contains, *],
   { simp },
-  any_goals {
-    /- Solve minor premises h₂ and h₅ -/
-    cases hs,
-    apply iff.intro,
+  twice { -- red and black cases are identical
     {
-      intro hm, blast_disjs,
-      { exact iff.mp (ih hs₁) hm },
-      { contradiction },
+      cases hs,
+      apply iff.intro,
       {
-        have hyx : lift lt (some y) (some x) := (range hs₂ hm).1,
-        simp [lift] at hyx,
-        have hxy : lt x y, { simp [cmp_using] at h, assumption },
-        exact absurd (trans_of lt hxy hyx) (irrefl_of lt x)
-      }
+        intro hm, blast_disjs,
+        { exact iff.mp (ih hs₁) hm },
+        { contradiction },
+        {
+          have hyx : lift lt (some y) (some x) := (range hs₂ hm).1,
+          simp [lift] at hyx,
+          have hxy : lt x y, { simp [cmp_using] at h, assumption },
+          exact absurd (trans_of lt hxy hyx) (irrefl_of lt x)
+        }
+      },
+      { intro hc, left, exact iff.mpr (ih hs₁) hc },
     },
-    { intro hc, left, exact iff.mpr (ih hs₁) hc },
-    done
- },
- any_goals {
-    /- Solve minor premises h₃ and h₆ -/
-    simp, done
- },
- any_goals {
-   /- Solve minor premises h₄ and h₇ -/
-   cases hs,
-   apply iff.intro,
-   {
-     intro hm, blast_disjs,
-     {
-       have hxy : lift lt (some x) (some y) := (range hs₁ hm).2,
-       simp [lift] at hxy,
-       have hyx : lt y x, { simp [cmp_using] at h, exact h.1 },
-       exact absurd (trans_of lt hxy hyx) (irrefl_of lt x)
-     },
-     { contradiction },
-     { exact iff.mp (ih hs₂) hm }
-   },
-   { intro hc, right, right, exact iff.mpr (ih hs₂) hc },
-   done
- }
+    { simp, done },
+    {
+      cases hs,
+      apply iff.intro,
+      {
+        intro hm, blast_disjs,
+        {
+          have hxy : lift lt (some x) (some y) := (range hs₁ hm).2,
+          simp [lift] at hxy,
+          have hyx : lt y x, { simp [cmp_using] at h, exact h.1 },
+          exact absurd (trans_of lt hxy hyx) (irrefl_of lt x)
+        },
+        { contradiction },
+        { exact iff.mp (ih hs₂) hm }
+      },
+      { intro hc, right, right, exact iff.mpr (ih hs₂) hc },
+    } }
 end
 
 inductive is_red_black : rbnode α → color → nat → Prop
@@ -271,6 +238,39 @@ begin
  apply le_trans, apply depth_max h, apply this
 end
 
+section
+open tactic
+meta def is_searchable_constructor_app : expr → bool
+| `(is_searchable _ leaf _ _)               := tt
+| `(is_searchable _ (red_node _ _ _) _ _)   := tt
+| `(is_searchable _ (black_node _ _ _) _ _) := tt
+| _                                         := ff
+
+meta def apply_is_searchable_constructors : tactic unit :=
+repeat $ any_goals $ do
+  t ← target,
+  guard $ is_searchable_constructor_app t,
+  constructor
+
+meta def destruct_is_searchable_hyps : tactic unit :=
+repeat $ any_goals $ any_hyp $ λ h, do
+  t ← infer_type h,
+  guard $ is_searchable_constructor_app t,
+  cases h,
+  clear h
+
+meta def is_searchable_tactic : tactic unit :=
+destruct_is_searchable_hyps; apply_is_searchable_constructors; try assumption
+
+end
+
+lemma balance1_searchable {l r t : rbnode α} {y v : α} {lt : α → α → Prop} {lo hi}
+                          : is_searchable lt l lo (some y) → is_searchable lt r (some y) (some v) → is_searchable lt t (some v) hi → is_searchable lt (balance1 l y r v t) lo hi :=
+begin
+  cases l; cases r; intros; simp [balance1],
+  all_goals { is_searchable_tactic }
+end
+
 lemma balance1_rb {l r t : rbnode α} {y v : α} {c_l c_r c_t n} : is_red_black l c_l n → is_red_black r c_r n → is_red_black t c_t n → ∃ c, is_red_black (balance1 l y r v t) c (succ n) :=
 begin
   intros h₁ h₂ h₃, cases h₁; cases h₂; repeat {assumption <|> constructor},
@@ -312,14 +312,14 @@ variables (lt : α → α → Prop) [decidable_rel lt]
 lemma ins.induction {p : rbnode α → Prop}
   (t x)
   (h₁ : p leaf)
-  (h₂ : ∀ a y b, cmp_using lt x y = ordering.lt → p a → p (red_node a y b))
-  (h₃ : ∀ a y b, cmp_using lt x y = ordering.eq → p (red_node a y b))
-  (h₄ : ∀ a y b, cmp_using lt x y = ordering.gt → p b → p (red_node a y b))
-  (h₅ : ∀ a y b, cmp_using lt x y = ordering.lt → get_color a = red → p a → p (black_node a y b))
-  (h₆ : ∀ a y b, cmp_using lt x y = ordering.lt → get_color a ≠ red → p a → p (black_node a y b))
-  (h₇ : ∀ a y b, cmp_using lt x y = ordering.eq → p (black_node a y b))
-  (h₈ : ∀ a y b, cmp_using lt x y = ordering.gt → get_color b = red → p b → p (black_node a y b))
-  (h₉ : ∀ a y b, cmp_using lt x y = ordering.gt → get_color b ≠ red → p b → p (black_node a y b))
+  (h₂ : ∀ a y b (hc : cmp_using lt x y = ordering.lt) (ih : p a), p (red_node a y b))
+  (h₃ : ∀ a y b (hc : cmp_using lt x y = ordering.eq), p (red_node a y b))
+  (h₄ : ∀ a y b (hc : cmp_using lt x y = ordering.gt) (ih : p b), p (red_node a y b))
+  (h₅ : ∀ a y b (hc : cmp_using lt x y = ordering.lt) (hr : get_color a = red) (ih : p a), p (black_node a y b))
+  (h₆ : ∀ a y b (hc : cmp_using lt x y = ordering.lt) (hnr : get_color a ≠ red) (ih : p a), p (black_node a y b))
+  (h₇ : ∀ a y b (hc : cmp_using lt x y = ordering.eq), p (black_node a y b))
+  (h₈ : ∀ a y b (hc : cmp_using lt x y = ordering.gt) (hr : get_color b = red) (ih : p b), p (black_node a y b))
+  (h₉ : ∀ a y b (hc : cmp_using lt x y = ordering.gt) (hr : get_color b ≠ red) (ih : p b), p (black_node a y b))
   : p t :=
 begin
   induction t,
@@ -346,6 +346,106 @@ begin
        { apply h₉, assumption, assumption, assumption },
      }
   }
+end
+
+lemma is_searchable_of_is_searchable_of_incomp [is_strict_weak_order α lt] {t} : ∀ {lo hi hi'} (hc : ¬ lt hi' hi ∧ ¬ lt hi hi') (hs : is_searchable lt t lo (some hi)), is_searchable lt t lo (some hi') :=
+begin
+  induction t; intros; is_searchable_tactic,
+  { cases lo; simp [lift, *] at *, apply lt_of_lt_of_incomp, assumption, assumption },
+  twice { apply ih_2 hc hs₂ }
+end
+
+lemma is_searchable_of_incomp_of_is_searchable [is_strict_weak_order α lt] {t} : ∀ {lo lo' hi} (hc : ¬ lt lo' lo ∧ ¬ lt lo lo') (hs : is_searchable lt t (some lo) hi), is_searchable lt t (some lo') hi :=
+begin
+  induction t; intros; is_searchable_tactic,
+  { cases hi; simp [lift, *] at *, cases hc, apply lt_of_incomp_of_lt, split, assumption, assumption, assumption },
+  twice { apply ih_1 hc hs₁ }
+end
+
+lemma is_searchable_some_low_of_is_searchable_of_lt {t} [is_trans α lt] : ∀ {lo hi lo'} (hlt : lt lo' lo) (hs : is_searchable lt t (some lo) hi), is_searchable lt t (some lo') hi :=
+begin
+  induction t; intros; is_searchable_tactic,
+  { cases hi; simp [lift, *] at *, apply trans_of lt hlt, assumption },
+  twice { apply ih_1 hlt hs₁ }
+end
+
+lemma is_searchable_none_low_of_is_searchable_some_low {t} : ∀ {y hi} (hlt : is_searchable lt t (some y) hi), is_searchable lt t none hi :=
+begin
+  induction t; intros; is_searchable_tactic,
+  { simp [lift] },
+  twice { apply ih_1 hs₁ }
+end
+
+lemma is_searchable_some_high_of_is_searchable_of_lt {t} [is_trans α lt] : ∀ {lo hi hi'} (hlt : lt hi hi') (hs : is_searchable lt t lo (some hi)), is_searchable lt t lo (some hi') :=
+begin
+  induction t; intros; is_searchable_tactic,
+  { cases lo; simp [lift, *] at *, apply trans_of lt, assumption, assumption},
+  twice { apply ih_2 hlt hs₂ }
+end
+
+lemma is_searchable_none_high_of_is_searchable_some_high {t} : ∀ {lo y} (hlt : is_searchable lt t lo (some y)), is_searchable lt t lo none :=
+begin
+  induction t; intros; is_searchable_tactic,
+  { cases lo; simp [lift] },
+  twice { apply ih_2 hs₂ }
+end
+
+lemma is_searchable_balance1 {l y r v t lo hi} (hl : is_searchable lt l lo (some y)) (hr : is_searchable lt r (some y) (some v)) (ht : is_searchable lt t (some v) hi) : is_searchable lt (balance1 l y r v t) lo hi :=
+by cases l; cases r; simp [balance1]; is_searchable_tactic
+
+lemma is_searchable_balance1_node {t} [is_trans α lt] : ∀ {y s lo hi}, is_searchable lt t lo (some y) → is_searchable lt s (some y) hi → is_searchable lt (balance1_node t y s) lo hi :=
+begin
+  cases t; simp [balance1_node]; intros; is_searchable_tactic,
+  { cases lo,
+    { apply is_searchable_none_low_of_is_searchable_some_low, assumption },
+    { simp [lift] at *, apply is_searchable_some_low_of_is_searchable_of_lt, assumption, assumption } },
+  twice { apply is_searchable_balance1, repeat { assumption } }
+end
+
+lemma is_searchable_balance2 {l y r v t lo hi} (ht : is_searchable lt t lo (some v)) (hl : is_searchable lt l (some v) (some y)) (hr : is_searchable lt r (some y) hi) : is_searchable lt (balance2 l y r v t) lo hi :=
+by cases l; cases r; simp [balance2]; is_searchable_tactic
+
+lemma is_searchable_balance2_node {t} [is_trans α lt] : ∀ {y s lo hi}, is_searchable lt s lo (some y) → is_searchable lt t (some y) hi → is_searchable lt (balance2_node t y s) lo hi :=
+begin
+  induction t; simp [balance2_node]; intros; is_searchable_tactic,
+  { cases hi,
+    { apply is_searchable_none_high_of_is_searchable_some_high, assumption },
+    { simp [lift] at *, apply is_searchable_some_high_of_is_searchable_of_lt, assumption, assumption } },
+  twice { apply is_searchable_balance2, repeat { assumption } }
+end
+
+lemma is_searchable_ins {t x} [is_strict_weak_order α lt] : ∀ {lo hi} (h : is_searchable lt t lo hi), lift lt lo (some x) → lift lt (some x) hi → is_searchable lt (ins lt t x) lo hi :=
+begin
+  apply ins.induction lt t x; intros; simp [ins, lift, *] at * {eta := ff}; is_searchable_tactic,
+  { apply ih hs₁, assumption, simp [lift, *] },
+  { apply is_searchable_of_is_searchable_of_incomp lt hc, assumption },
+  { apply is_searchable_of_incomp_of_is_searchable lt hc, assumption },
+  { apply ih hs₂, cases hi; simp [lift, *], assumption },
+  { apply is_searchable_balance1_node, apply ih hs₁, assumption, simp [lift, *], assumption },
+  { apply ih hs₁, assumption, simp [lift, *] },
+  { apply is_searchable_of_is_searchable_of_incomp lt hc, assumption },
+  { apply is_searchable_of_incomp_of_is_searchable lt hc, assumption },
+  { apply is_searchable_balance2_node, assumption, apply ih hs₂, simp [lift, *], assumption },
+  { apply ih hs₂, assumption, simp [lift, *] }
+end
+
+lemma is_searchable_flip_red {t} : is_searchable lt t none none → is_searchable lt (flip_red t) none none :=
+begin
+  cases t; simp [flip_red],
+  any_goals { exact id },
+  { intro h, is_searchable_tactic }
+end
+
+lemma is_searchable_insert {t x} [is_strict_weak_order α lt] : is_searchable lt t none none → is_searchable lt (insert lt t x) none none :=
+begin
+  intro h, simp [insert], apply is_searchable_flip_red, apply is_searchable_ins, assumption, simp [lift], simp [lift]
+end
+
+lemma is_searchable_of_well_formed {t : rbnode α } [is_strict_weak_order α lt] : t.well_formed lt → is_searchable lt t none none :=
+begin
+  intro h, induction h,
+  { constructor, simp [lift] },
+  { subst n', apply is_searchable_insert, assumption }
 end
 
 end insert
@@ -422,7 +522,7 @@ begin
   simp [insert],
   have h : ins lt t a ≠ leaf, { apply ins_ne_leaf },
   generalize he : ins lt t a = r,
-  cases r; simp [insert],
+  cases r; simp [flip_red, insert],
   case leaf { contradiction },
   case black_node { rw [←he], apply mem_ins },
   case red_node {
